Computability/playground.lean
@@ -1,4 +1,5 @@
 import Computability.Constructions
+
 open Nat
 
 -- theorem h0' (h:x>0): x-1+1=x := by exact Nat.sub_add_cancel h
@@ -7,4 +8,8 @@ open Nat
 --   simp only [reduceEqDiff, ↓reduceIte]ℕ 
 
 -- theorem asd : ¬ (s+1=0) := by exact add_one_ne_zero s
-theorem asd (h:x>0): x-1+1=x := by exact Nat.sub_add_cancel h
+-- theorem asd (h:x>0): x-1+1=x := by exact Nat.sub_add_cancel h
+-- have asd:n%2≤1 := by exact?
+theorem bounds_aux_2 : Nat.pair m.l (s + 1) < Nat.pair (n + 4 + 1) (s + 1) := by
+      exact pair_lt_pair_left (s+1) bounds_aux_1
+have bounds : Nat.pair m.l (s + 1) ≤ k := by
